\begin{problem}[L 2.4.2]
  Use the method of exercise 2.4.2 to compute numerical solutions of the scalar initial value problem $y' = 4xy^{1/2}$, $y(0) = 1$ for $0 \leq x \leq 2$, using the steplengths $h = 0.1$, $0.05$, and $0.025$. Compare the results with the exact solution $y(x) = (1 + x^2)^2$ and deduce that the numerical solutions are not converging to the exact solution as $h \to 0$.
\end{problem}

\begin{solution}
  We are using the method
  \[
    y_{n + 2} - y_{n + 1} = \frac{h}{12}\left[4 f(x_{n + 2}, y_{n + 2}) + 8 f(x_{n + 1}, y_{n + 1}) - f(x_n, y_n)\right].
  \]
  In this case, $f(x, y) = 4xy^{1/2}$, and $x_n = nh$. We can use this to simplify the method. After a bit of computation, we have
  \[
    \frac{4}{3} (n + 2) h^2 \sqrt{y_{n + 2}} = y_{n + 2} + \frac{1}{3} n h^2 y_n^{1/2} - \frac{8}{3} (n + 1) h^2 y_{n + 1}^{1/2} - y_{n + 1}.
  \]
  Let
  \begin{align*}
    A &= \frac{4}{3} (n + 2) h^2 \\
    B &= \frac{1}{3} n h^2 y_n^{1/2} - \frac{8}{3} (n + 1) h^2 y_{n + 1}^{1/2} - y_{n + 1}.
  \end{align*}
  Then we can simplify to
  \[
    0 = y_{n+2}^2 + (2B - A^2)y_{n+2} + B^2.
  \]
  Writing 
  \begin{align*}
    C &= 2B - A^2 \\
    D &= B^2
  \end{align*}
  we can simplify and solve for $y_{n+2}$. We get
  \[
    y_{n + 2} = \frac{-C + \sqrt{C^2 - 4D}}{2}.
  \]
  We use this to solve the problem numerically for $h = 0.1$, $0.05$, and $0.025$.
  
  \begin{figure}[!ht]
    \centering
    \includegraphics[scale=0.3]{../plot/plot_1_1.png}
    \includegraphics[scale=0.3]{../plot/plot_1_2.png}
    \includegraphics[scale=0.3]{../plot/plot_1_3.png}
    \caption{$h = 0.1$, $h = 0.05$, $h = 0.025$}
    \label{fig:prob1}
  \end{figure}
  
  Figure \ref{fig:prob1} shows the numerical solutions for the different $h$ values compared with the actual solution of $y(x) = (1+x^2)^2$. It is obvious from the images that the numerical solution is converging, but not to the  actual solution.
  
  We can see why this is happening by analyzing the consistency of the method. The characteristic polynomial associated with the method is $\rho(\zeta) = \zeta^2 - \zeta$. Then $\rho'(1) = 1$. We know
  \[
    \phi_f(y_{n+2}, y_{n+1}, y_n, x_n; h) = \frac{1}{12}(4f(x_{n+2},y_{n+2}) + 8f(x_{n+1}, y_{n+1}) - f(x_n, y_n)).
  \]
  
  Thus, we have that
  \begin{align*}
    \phi_f(y(x_n), y(x_n), y(x_n), x_n; 0)/\rho'(1)
    &= \tfrac{1}{12}(4f(x_n,y(x_n)) + 8f(x_n, y(x_n)) - f(x_n, y(x_n))) \\
    &= \tfrac{11}{12}f(x_n,y(x_n)).
  \end{align*}
  
  Since $\phi_f(y(x_n), y(x_n), y(x_n), x_n; 0)/\rho'(1) \neq f(x_n,y(x_n))$, the method is not consistent and the numerical solutions are not converging to the exact solution as $h \to 0$.
\end{solution}
